\documentclass{article}
\usepackage{amsmath}
\begin{document}
$$(-2x^{2}y^{2}z+4xyz^{2}-2x^{2}yz) / (x y z) = (-8xy+8z-4x)$$
$$(-2x^{2}y^{2}z+4xy) + (+6xy+5z) = (-2x^{2}y^{2}z+10xy+5z)$$
$$(-2x^{2}y^{2}z+4xy) - (+6xy+5z) = (-2x^{2}y^{2}z-2xy-5z)$$
$$(-2x^{2}y^{2}z+4xy) * (+6xy+5t) = (-12x^{3}y^{3}z-10tx^{2}y^{2}z+24x^{2}y^{2}+20txy)$$
$$uniformity(-2x^{2}y^{2}z+4xyz^{3}) = 1$$
$$harmonicity(-2x^{2}y^{2}z+4xyz) = 0$$
$$(-2x^{2}y^{2}z+4xy) == (+6xy+5z) = 0$$
$$(-2x^{2}y^{2}z+4xy) != (+6xy+5z) = 1$$
$$(-2x^{2}y^{2}z+4xyz^{2}-2x^{2}yz) / (z) = (-2x^{2}y^{2}+8xyz-2x^{2}y)$$
\end{document}